PREFIX : <http://def.isotc211.org/iso19115/-1/2014/IdentificationInformation/code/MD_TopicCategoryCode/>
PREFIX astatus: <https://linked.data.gov.au/def/reg-statuses/>
PREFIX cs: <http://def.isotc211.org/iso19115/-1/2014/IdentificationInformation/code/MD_TopicCategoryCode>
PREFIX prov: <http://www.w3.org/ns/prov#>
PREFIX rdfs: <http://www.w3.org/2000/01/rdf-schema#>
PREFIX reg: <http://purl.org/linked-data/registry#>
PREFIX schema: <https://schema.org/>
PREFIX skos: <http://www.w3.org/2004/02/skos/core#>
PREFIX this-cs: <https://linked.data.gov.au/def/mer-topic-categories>
PREFIX xsd: <http://www.w3.org/2001/XMLSchema#>

<https://linked.data.gov.au/org/tc211>
    a schema:Organization ;
    schema:description "The International Organization for Standardization's Technical Committee on \"Geographic information/Geomatics\", charged with standardization in the field of digital geographic information"@en ;
    schema:name "ISO's Technical Committee 211" ;
    schema:url "https://www.iso.org/committee/54904.html"^^xsd:anyURI ;
.

:boundaries
    a skos:Concept ;
    reg:status astatus:original ;
    rdfs:isDefinedBy cs: ;
    skos:definition """Legal land descriptions.

Examples: political and administrative boundaries"""@en ;
    skos:inScheme this-cs: ;
    skos:prefLabel "Boundaries"@en ;
    skos:topConceptOf this-cs: ;
    schema:citation "Presented in the original standard's codelist"@en ;
.

:environment
    a skos:Concept ;
    reg:status astatus:original ;
    rdfs:isDefinedBy cs: ;
    skos:definition """Environmental resources, protection and conservation.

Examples: environmental pollution, waste storage and treatment, environmental impact assessment, monitoring environmental risk, nature reserves, landscape
    """@en ;
    skos:inScheme this-cs: ;
    skos:prefLabel "Environment"@en ;
    skos:topConceptOf this-cs: ;
    schema:citation "Presented in the original standard's codelist"@en ;
.

:geoscientificInformation
    a skos:Concept ;
    reg:status astatus:original ;
    rdfs:isDefinedBy cs: ;
    skos:definition """Information pertaining to earth sciences.

Examples: geophysical features and processes, geology, minerals, sciences dealing with the composition, structure and origin of the earth s rocks, risks of earthquakes, volcanic activity, landslides, gravity information, soils, permafrost, hydrogeology, erosion"""@en ;
    skos:inScheme this-cs: ;
    skos:prefLabel "Geoscientific Information"@en ;
    skos:topConceptOf this-cs: ;
    schema:citation "Presented in the original standard's codelist"@en ;
.

:transportation
    a skos:Concept ;
    reg:status astatus:original ;
    rdfs:isDefinedBy cs: ;
    skos:definition """Means and aids for conveying persons and/or goods.

Examples: roads, airports/airstrips, shipping routes, tunnels, nautical charts, vehicle or vessel location, aeronautical charts, railways"""@en ;
    skos:inScheme this-cs: ;
    skos:prefLabel "Transportation"@en ;
    skos:topConceptOf this-cs: ;
    schema:citation "Presented in the original standard's codelist"@en ;
.

:utilitiesCommunication
    a skos:Concept ;
    reg:status astatus:original ;
    rdfs:isDefinedBy cs: ;
    skos:definition """Energy, water and waste systems and communications infrastructure and services.

Examples: hydroelectricity, geothermal, solar and nuclear sources of energy, water purification and distribution, sewage collection and disposal, electricity and gas distribution, data communication, telecommunication, radio, communication networks"""@en ;
    skos:inScheme this-cs: ;
    skos:prefLabel "Utilities Communication"@en ;
    skos:topConceptOf this-cs: ;
    schema:citation "Presented in the original standard's codelist"@en ;
.

<https://linked.data.gov.au/org/mer>
    a schema:Organization ;
    schema:name "SA Minerals & Energy Resources" ;
    schema:url "https://www.energymining.sa.gov.au/industry/geological-survey"^^xsd:anyURI ;
.

this-cs:
    a skos:ConceptScheme ;
    reg:status astatus:stable ;
    skos:changeNote "2024-08-26 NJC Made VocPub 4.10 valid, LongTurtle formatted, no content changes" ;
    skos:definition "High-level geographic data thematic classification to assist in the grouping and search of available geographic datasets"@en ;
    skos:hasTopConcept
        :boundaries ,
        :environment ,
        :geoscientificInformation ,
        :transportation ,
        :utilitiesCommunication ;
    skos:prefLabel "Topic Categories"@en ;
    prov:qualifiedDerivation
        [
            prov:entity cs: ;
            prov:hadRole <https://linked.data.gov.au/def/vocab-derivation-modes/subsetting> ;
        ] ;
    schema:citation "Derived from http://def.isotc211.org/iso19115/-1/2014/IdentificationInformation/code/MD_TopicCategoryCode"@en ;
    schema:creator <https://linked.data.gov.au/org/mer> ;
    schema:dateCreated "2022-12-04"^^xsd:date ;
    schema:dateModified "2024-08-26"^^xsd:date ;
    schema:issued "2022-12-04"^^xsd:date ;
    schema:license <https://purl.org/NET/rdflicense/cc-by4.0> ;
    schema:publisher <https://linked.data.gov.au/org/mer> ;
    schema:rights "Â© Department for Energy and Mining, 2022"@en ;
.
