PREFIX : <https://linked.data.gov.au/def/vocdermods/>
PREFIX astatus: <https://linked.data.gov.au/def/reg-statuses/>
PREFIX cs: <https://linked.data.gov.au/def/vocdermods>
PREFIX rdfs: <http://www.w3.org/2000/01/rdf-schema#>
PREFIX reg: <http://purl.org/linked-data/registry#>
PREFIX schema: <https://schema.org/>
PREFIX skos: <http://www.w3.org/2004/02/skos/core#>
PREFIX xsd: <http://www.w3.org/2001/XMLSchema#>

:subsetting-and-extension
    a skos:Concept ;
    schema:citation "Created for the MER catalogue upgrade project, 2022"@en ;
    reg:status astatus:original ;
    rdfs:isDefinedBy cs: ;
    skos:broader
        :extension ,
        :subsetting ;
    skos:definition "Derivation with subsetting and extension"@en ;
    skos:inScheme cs: ;
    skos:prefLabel "Subset & Extension"@en ;
    skos:scopeNote "Use this Concept if the reusing vocabulary both extends and subsets the original vocabulary" ;
.

<https://kurrawong.ai>
    a schema:Organization ;
    schema:name "KurrawongAI" ;
    schema:url "https://kurrawong.ai"^^xsd:anyURI ;
.

:direct
    a skos:Concept ;
    schema:citation "Created for the MER catalogue upgrade project, 2022"@en ;
    reg:status astatus:original ;
    rdfs:isDefinedBy cs: ;
    skos:definition "Derivation without alteration"@en ;
    skos:inScheme cs: ;
    skos:prefLabel "Direct"@en ;
    skos:topConceptOf cs: ;
.

:none
    a skos:Concept ;
    schema:citation "Added to this vocabulary for multiple projects in 2023"@en ;
    reg:status astatus:original ;
    rdfs:isDefinedBy cs: ;
    skos:definition "This vocabulary does not derive from another"@en ;
    skos:inScheme cs: ;
    skos:prefLabel "None"@en ;
    skos:scopeNote "Use this Concept if the vocabulary is known to not reuse any other vocabularies" ;
    skos:topConceptOf cs: ;
.

:not-applicable
    a skos:Concept ;
    schema:citation "Created for the MER catalogue upgrade project, 2022"@en ;
    reg:status astatus:original ;
    rdfs:isDefinedBy cs: ;
    skos:definition "Derivation mode is not applicable to this vocabulary"@en ;
    skos:inScheme cs: ;
    skos:prefLabel "Not Applicable"@en ;
    skos:scopeNote "Use this Concept if the vocabulary is known not to reuse any other vocabularies" ;
    skos:topConceptOf cs: ;
.

:relabelling
    a skos:Concept ;
    schema:citation "Created for the MER catalogue upgrade project, 2022"@en ;
    reg:status astatus:original ;
    rdfs:isDefinedBy cs: ;
    skos:definition "Derivation with relabelling"@en ;
    skos:inScheme cs: ;
    skos:prefLabel "Relabelling"@en ;
    skos:scopeNote "Use this Concept if the reusing vocabulary only relabels Concepts in the original vocabulary but does not alter their place in the Concept hierarchy or their definitions" ;
    skos:topConceptOf cs: ;
.

<https://linked.data.gov.au/org/agldwg>
    a schema:Organization ;
    schema:name "Australian Government Linked Data Working Group" ;
    schema:url "https://www.linked.data.gov.au"^^xsd:anyURI ;
.

:extension
    a skos:Concept ;
    schema:citation "Created for the MER catalogue upgrade project, 2022"@en ;
    reg:status astatus:original ;
    rdfs:isDefinedBy cs: ;
    skos:definition "Derivation with extension"@en ;
    skos:inScheme cs: ;
    skos:prefLabel "Extension"@en ;
    skos:scopeNote "Use this Concept if the reusing vocabulary extends the original vocabulary but does not subset it" ;
    skos:topConceptOf cs: ;
.

:subsetting
    a skos:Concept ;
    schema:citation "Created for the MER catalogue upgrade project, 2022"@en ;
    reg:status astatus:original ;
    rdfs:isDefinedBy cs: ;
    skos:definition "Derivation with subsetting"@en ;
    skos:inScheme cs: ;
    skos:prefLabel "Subsetting"@en ;
    skos:scopeNote "Use this Concept if the reusing vocabulary only subsets the original but does not extend it" ;
    skos:topConceptOf cs: ;
.

cs:
    a skos:ConceptScheme ;
    schema:dateCreated "2022-12-05"^^xsd:date ;
    schema:creator <https://kurrawong.ai> ;
    schema:issued "2022-12-05"^^xsd:date ;
    schema:dateModified "2024-08-26"^^xsd:date ;
    schema:citation "Created for the MER catalogue upgrade project, 2022"@en ;
    schema:publisher <https://linked.data.gov.au/org/agldwg> ;
    reg:status astatus:stable ;
    skos:definition "The modes by which one vocabulary may derive from another"@en ;
    skos:hasTopConcept
        :direct ,
        :extension ,
        :none ,
        :not-applicable ,
        :relabelling ,
        :subsetting ;
    skos:prefLabel "Vocabulary Derivation Modes"@en ;
.
